simplify

src/3d/prelude/EverParse3d.Serializer.fst
@@ -5,17 +5,17 @@ open LowParse.Spec.Combinators
 
 let in_codomain p x = exists y. p y == Some (x, Seq.length y)
 
-let serialize p x = FStar.IndefiniteDescription.indefinite_description_ghost bytes (fun y -> p y == Some (x, Seq.length y))
+let serialize p x = IndefiniteDescription.indefinite_description_ghost bytes (fun y -> p y == Some (x, Seq.length y))
 
-let serializes_to_intro p x b = LowParse.Spec.Base.parse_injective p (serialize p x) b
+let serializes_to_iff p x b =
+  introduce p b == Some (x, Seq.length b) ==> serializes_to p x b with _.
+    LowParse.Spec.Base.parse_injective p (serialize p x) b
 
-let serialize_inj p x1 x2 = serializes_to_intro p x1 (serialize p x2)
+let serialize_inj p x1 x2 = ()
 
-let serializes_to_ret v = serializes_to_intro (parse_ret v) v Seq.empty
+let serializes_to_ret v = ()
 
-let serializes_to_filter p f x =
-  parse_filter_eq p f (serialize p x);
-  serializes_to_intro (parse_filter p f) x (serialize p x)
+let serializes_to_filter p f x = parse_filter_eq p f (serialize p x)
 
 let in_codomain_filter p f x =
   introduce in_codomain (parse_filter p f) x ==> in_codomain p x with _.
@@ -27,8 +27,7 @@ let serializes_to_dtuple2 p1 p2 x1 x2 =
   let b2 = serialize (p2 x1) x2 in
   LowParse.Spec.Base.parse_strong_prefix p1 b1 (Seq.append b1 b2);
   LowParse.Spec.Combinators.parse_dtuple2_eq p1 p2 (Seq.append b1 b2);
-  FStar.Seq.Properties.append_slices b1 b2;
-  serializes_to_intro (parse_dtuple2 p1 p2) (| x1, x2 |) (Seq.append b1 b2)
+  Seq.append_slices b1 b2
 
 let in_codomain_dtuple2 p1 p2 x1 x2 =
   introduce in_codomain p1 x1 /\ in_codomain (p2 x1) x2 ==> in_codomain (parse_dtuple2 p1 p2) (| x1, x2 |) with _. serializes_to_dtuple2 p1 p2 x1 x2;
@@ -37,8 +36,7 @@ let in_codomain_dtuple2 p1 p2 x1 x2 =
     LowParse.Spec.Combinators.parse_dtuple2_eq p1 p2 b;
     let Some (x1', c1) = p1 b in
     let b1 = Seq.slice b 0 c1 in
-    LowParse.Spec.Base.parse_strong_prefix p1 b b1;
-    serializes_to_intro p1 x1 b1
+    LowParse.Spec.Base.parse_strong_prefix p1 b b1
   end
 
 let serializes_to_nondep_then p1 p2 x1 x2 =
@@ -46,8 +44,7 @@ let serializes_to_nondep_then p1 p2 x1 x2 =
   let b2 = serialize p2 x2 in
   LowParse.Spec.Base.parse_strong_prefix p1 b1 (Seq.append b1 b2);
   LowParse.Spec.Combinators.nondep_then_eq p1 p2 (Seq.append b1 b2);
-  FStar.Seq.Properties.append_slices b1 b2;
-  serializes_to_intro (nondep_then p1 p2) (x1, x2) (Seq.append b1 b2)
+  Seq.append_slices b1 b2
 
 let in_codomain_nondep_then p1 p2 x1 x2 =
   introduce in_codomain p1 x1 /\ in_codomain p2 x2 ==> in_codomain (nondep_then p1 p2) (x1, x2) with _. serializes_to_nondep_then p1 p2 x1 x2;
@@ -56,50 +53,39 @@ let in_codomain_nondep_then p1 p2 x1 x2 =
     LowParse.Spec.Combinators.nondep_then_eq p1 p2 b;
     let Some (x1', c1) = p1 b in
     let b1 = Seq.slice b 0 c1 in
-    LowParse.Spec.Base.parse_strong_prefix p1 b b1;
-    serializes_to_intro p1 x1 b1
+    LowParse.Spec.Base.parse_strong_prefix p1 b b1
   end
 
 let serializes_to_u8 x =
-  LowParse.Spec.Int.parse_u8_spec (Endianness.n_to_be 1 (UInt8.v x));
-  serializes_to_intro LowParse.Spec.Int.parse_u8 x (Endianness.n_to_be 1 (UInt8.v x))
+  LowParse.Spec.Int.parse_u8_spec (Endianness.n_to_be 1 (UInt8.v x))
 
 let serializes_to_u16be x =
-  LowParse.Spec.Int.parse_u16_spec (Endianness.n_to_be 2 (UInt16.v x));
-  serializes_to_intro LowParse.Spec.Int.parse_u16 x (Endianness.n_to_be 2 (UInt16.v x))
+  LowParse.Spec.Int.parse_u16_spec (Endianness.n_to_be 2 (UInt16.v x))
 
 let serializes_to_u32be x =
-  LowParse.Spec.Int.parse_u32_spec (Endianness.n_to_be 4 (UInt32.v x));
-  serializes_to_intro LowParse.Spec.Int.parse_u32 x (Endianness.n_to_be 4 (UInt32.v x))
+  LowParse.Spec.Int.parse_u32_spec (Endianness.n_to_be 4 (UInt32.v x))
 
 let serializes_to_u64be x =
-  LowParse.Spec.Int.parse_u64_spec (Endianness.n_to_be 8 (UInt64.v x));
-  serializes_to_intro LowParse.Spec.Int.parse_u64 x (Endianness.n_to_be 8 (UInt64.v x))
+  LowParse.Spec.Int.parse_u64_spec (Endianness.n_to_be 8 (UInt64.v x))
 
 let serializes_to_u16le x =
-  LowParse.Spec.BoundedInt.parse_u16_le_spec (Endianness.n_to_le 2 (UInt16.v x));
-  serializes_to_intro LowParse.Spec.BoundedInt.parse_u16_le x (Endianness.n_to_le 2 (UInt16.v x))
+  LowParse.Spec.BoundedInt.parse_u16_le_spec (Endianness.n_to_le 2 (UInt16.v x))
 
 let serializes_to_u32le x =
-  LowParse.Spec.BoundedInt.parse_u32_le_spec (Endianness.n_to_le 4 (UInt32.v x));
-  serializes_to_intro LowParse.Spec.BoundedInt.parse_u32_le x (Endianness.n_to_le 4 (UInt32.v x))
+  LowParse.Spec.BoundedInt.parse_u32_le_spec (Endianness.n_to_le 4 (UInt32.v x))
 
 let serializes_to_u64le x =
-  LowParse.Spec.Int.parse_u64_le_spec (Endianness.n_to_le 8 (UInt64.v x));
-  serializes_to_intro LowParse.Spec.Int.parse_u64_le x (Endianness.n_to_le 8 (UInt64.v x))
+  LowParse.Spec.Int.parse_u64_le_spec (Endianness.n_to_le 8 (UInt64.v x))
 
-let serializes_to_fldata p sz x =
-  serializes_to_intro (parse_fldata p sz) x (serialize p x)
+let serializes_to_fldata p sz x = ()
 
 let in_codomain_fldata p sz x =
   introduce in_codomain (parse_fldata p sz) x ==> in_codomain p x /\ Seq.length (serialize p x) == sz with _.
-    serializes_to_intro p x (serialize (parse_fldata p sz) x);
+    serializes_to_iff p x (serialize (parse_fldata p sz) x);
   introduce in_codomain p x /\ Seq.length (serialize p x) == sz ==> in_codomain (parse_fldata p sz) x with _.
     serializes_to_fldata p sz x
 
-let serializes_to_list_nil p =
-  parse_list_eq p Seq.empty;
-  serializes_to_intro (parse_list p) [] Seq.empty
+let serializes_to_list_nil p = parse_list_eq p Seq.empty
 
 let serializes_to_list_cons p x xs =
   let b1 = serialize p x in
@@ -107,8 +93,7 @@ let serializes_to_list_cons p x xs =
   let bs = Seq.append b1 b2 in
   LowParse.Spec.Base.parse_strong_prefix p b1 bs;
   parse_list_eq p bs;
-  Seq.append_slices b1 b2;
-  serializes_to_intro (parse_list p) (x::xs) bs
+  Seq.append_slices b1 b2
 
 let in_codomain_list_cons p x xs =
   introduce in_codomain (parse_list p) (x::xs) ==>
@@ -118,7 +103,7 @@ let in_codomain_list_cons p x xs =
     parse_list_eq p bs;
     let Some (x', n) = p bs in
     LowParse.Spec.Base.parse_strong_prefix p bs (Seq.slice bs 0 n);
-    serializes_to_intro p x (Seq.slice bs 0 n)
+    serializes_to_iff p x (Seq.slice bs 0 n)
   end;
   introduce in_codomain p x /\ Seq.length (serialize p x) > 0 /\ in_codomain (parse_list p) xs ==>
       in_codomain (parse_list p) (x::xs) with _.
